coq.yalla/log_cut_elim.v
@@ -16,10 +16,9 @@ Require Import List_more List_Type_more Permutation_Type genperm_Type.
 Require Import orthogonality log_phase_sem.
 
 Require Import ill_def.
-
-Import SetNotations.
+Import SetNotations. (* ⊆ ≃ ∩ ∪ ∅ *)
 Definition ill_lbang := map ioc.
-Notation "‼ x" := (ill_lbang x) (at level 53).
+Notation "‼ x" := (ill_lbang x) (at level 55).
 
 
 Set Implicit Arguments.
@@ -53,8 +52,8 @@ Section SyntacticModel.
 
   Notation ctx_compose := (@app iformula).
   Notation ctx_unit := (@nil iformula).
-  Notation adj_l := (fun ϴ H => match H with (Γ,Δ,A) => (Γ, ϴ ++ Δ, A) end).
-  Notation adj_r := (fun ϴ H => match H with (Γ,Δ,A) => (Γ ++ ϴ, Δ, A) end).
+  Notation ctx_adj_l := (fun ϴ H => match H with (Γ,Δ,A) => (Γ, ϴ ++ Δ, A) end).
+  Notation ctx_adj_r := (fun ϴ H => match H with (Γ,Δ,A) => (Γ ++ ϴ, Δ, A) end).
 
   Notation ctx_hole := (list iformula * list iformula * iformula)%type.
   Infix "∘" := (composes ctx_compose) (at level 50, no associativity).
@@ -65,16 +64,33 @@ Section SyntacticModel.
   Instance CL_ctx : ClosureOp := (@lclosure _ _ ctx_orth).
   Notation cl_ctx := (@cl _ _ CL_ctx).
 
-  Lemma rel_associative_l_l : rel_associativity_l_l ctx_orth ctx_compose adj_r.
+  Lemma cl_ctx_to_logic ϴ ϴ' : cl (sg ϴ') ϴ -> forall Γ Δ A,
+    Γ ++ ϴ' ++ Δ ⊢ A [P] -> Γ ++ ϴ ++ Δ ⊢ A [P].
+  Proof.
+  unfold cl_ctx, CL_ctx, lclosure, ctx_orth, ldual, rdual.
+  intros Hcl Γ Δ A pi.
+  specialize Hcl with (Γ,Δ,A); apply Hcl.
+  intros x Hx; subst; assumption.
+  Qed.
+
+  Lemma logic_to_cl_ctx ϴ ϴ' : (forall Γ Δ A, Γ ++ ϴ' ++ Δ ⊢ A [P] -> Γ ++ ϴ ++ Δ ⊢ A [P]) ->
+    cl (sg ϴ') ϴ.
+  Proof.
+  unfold cl_ctx, CL_ctx, lclosure, ctx_orth, ldual, rdual.
+  intros Hlog [[Γ Δ] A] Hcl.
+  apply Hlog, Hcl; reflexivity.
+  Qed.
+
+  Lemma rel_associative_l_l : rel_associativity_l_l ctx_orth ctx_compose ctx_adj_r.
   Proof. intros X Y [[X1 Y1] A]; unfold ctx_orth; rewrite <- ? app_assoc; auto. Qed.
 
-  Lemma rel_associative_l_r : rel_associativity_l_r ctx_orth ctx_compose adj_r.
+  Lemma rel_associative_l_r : rel_associativity_l_r ctx_orth ctx_compose ctx_adj_r.
   Proof. intros X Y [[X1 Y1] A]; unfold ctx_orth; rewrite <- ? app_assoc; auto. Qed.
 
-  Lemma rel_associative_r_l : rel_associativity_r_l ctx_orth ctx_compose adj_l.
+  Lemma rel_associative_r_l : rel_associativity_r_l ctx_orth ctx_compose ctx_adj_l.
   Proof. intros X Y [[X1 Y1] A]; unfold ctx_orth; rewrite <- app_assoc; auto. Qed.
 
-  Lemma rel_associative_r_r : rel_associativity_r_r ctx_orth ctx_compose adj_l.
+  Lemma rel_associative_r_r : rel_associativity_r_r ctx_orth ctx_compose ctx_adj_l.
   Proof. intros X Y [[X1 Y1] A]; unfold ctx_orth; rewrite <- app_assoc; auto. Qed.
 
   Fact cl_comm : ipperm P = true -> @cl_commutativity _ _ CL_ctx (composes ctx_compose).
@@ -125,8 +141,8 @@ Section SyntacticModel.
   split; [ exists l0 | exists l1 ]; reflexivity.
   Qed.
 
-  Instance PS_ctx : MPhaseSpace (ipperm P) :=
-  { Web := list iformula;
+  Instance PS_ctx : MPhaseSpace (ipperm P) := {
+    Web := list iformula;
     PScompose := (@app iformula);
     PSunit := nil;
     PS_associative := (@app_assoc _);
@@ -144,14 +160,18 @@ Section SyntacticModel.
 
   Notation "↓" := (fun A Γ => Γ ⊢ A [P]).
 
-  Fact dc_closed A : cl (↓A) ⊆ ↓A.
+  Fact dc_closed A : cl(↓A) ⊆ ↓A.
   Proof.
   intros ga Hga; simpl in Hga; unfold ldual, rdual, ctx_orth in Hga.
-  replace ga with (nil++ga++nil) by (list_simpl; reflexivity).
   specialize Hga with (nil,nil,A).
+  replace ga with (nil++ga++nil) by (list_simpl; reflexivity).
   apply Hga.
-  intro; rewrite <- app_nil_end; auto.
+  intro; rewrite app_nil_r; auto.
   Qed.
+
+  Fact closure_sg_in_dc A : cl_ctx (sg (A :: nil)) ⊆ ↓A.
+  (* the converse ↓A ⊆ cl_ctx (sg (A :: nil)) is exactly cut *)
+  Proof. etransitivity; [ apply cl_monotone | apply dc_closed ]; apply sg_subset, ax_exp_ill. Qed.
 
   Hint Resolve subset_preorder dc_closed.
 
@@ -177,22 +197,20 @@ Section SyntacticModel.
   Qed.
 
   Fact ILLgax : forall a, list_form_presem PS_ctx (ILLval P) (fst (projT2 (ipgax P) a))
-                    ⊆ cl(form_presem PS_ctx (ILLval P) (snd (projT2 (ipgax P) a))).
+                          ⊆ cl(form_presem PS_ctx (ILLval P) (snd (projT2 (ipgax P) a))).
   Proof.
   intros.
   etransitivity; [ | apply cl_increase ].
-  destruct (atlist_from_gax a) as [l Heq].
-  rewrite Heq.
+  destruct (atlist_from_gax a) as [l Heq]; rewrite Heq.
   red in P_gax_at_r; specialize P_gax_at_r with a.
   remember (snd (projT2 (ipgax P) a)) as b.
   destruct b; inversion P_gax_at_r; subst.
   intros x Hx; right; rewrite Heqb.
   enough (forall l0 a l1 l2, map ivar l1 ++ map ivar l0 = fst (projT2 (ipgax P) a) ->
-            list_form_presem PS_ctx (ILLval P) (map £ l0) l2 ->
+            list_form_presem PS_ctx (ILLval P) (map ivar l0) l2 ->
             { c | map ivar l1 ++ l2 = fst (projT2 (ipgax P) c)
-               /\ snd (projT2 (ipgax P) a) = snd (projT2 (ipgax P) c) }).
-  { specialize X with l a nil x; list_simpl in X.
-    symmetry in Heq; apply X in Heq; auto. }
+               /\ snd (projT2 (ipgax P) a) = snd (projT2 (ipgax P) c) })
+    by (specialize X with l a nil x; list_simpl in X; symmetry in Heq; apply X in Heq; auto).
   clear - P_gax_at_l P_gax_cut; induction l0; intros a' l1 l2 Heq Hsem; inversion Hsem; subst.
   - list_simpl in Heq.
     exists a'; split; list_simpl; auto.
@@ -208,7 +226,7 @@ Section SyntacticModel.
       destruct Heq as [d [Heq3 Heq4]].
       destruct (atlist_from_gax c) as [l' Heq'].
       rewrite_all Heq'.
-      apply IHl0 with (a:=d) (l1 := l1 ++ l') in X0; list_simpl; auto.
+      apply IHl0 with (a := d) (l1 := l1 ++ l') in X0; list_simpl; auto.
       list_simpl in X0; destruct X0 as [e [Heq5 Heq6]].
       exists e; split; auto.
       etransitivity; eassumption.
@@ -219,18 +237,39 @@ Section SyntacticModel.
     PMval := ILLval P;
     PMgax := ILLgax }.
 
-  Infix "⊸" := (magicwand_l PScompose) (at level 51, right associativity).
-  Infix "⟜" := (magicwand_r PScompose) (at level 52, left associativity).
+  Infix "⊸" := (magicwand_l PScompose) (at level 52, right associativity).
+  Infix "⟜" := (magicwand_r PScompose) (at level 53, left associativity).
   Notation v := PMval.
-  Notation "⟦ A ⟧" := (form_presem PS_ctx (ILLval P) A) (at level 49).
+  Notation "⟦ A ⟧" := (form_presem PS_ctx (ILLval P) A).
+  Notation "⟬߭ Γ ⟭" := (list_form_presem PS_ctx (ILLval P) Γ).
+  Notation "□" := (@cl _ _ PSCL).
+  Notation "l ⊧  x" := (@list_compose _ PMPS l ⊆ x) (at level 70, no associativity).
 
   Hint Resolve (@PScl_stable_l _ PMPS) (@PScl_stable_r _ PMPS)
                magicwand_l_adj_l magicwand_l_adj_r magicwand_r_adj_l magicwand_r_adj_r.
+
+
+  Lemma logic_to_plogic ϴ ϴ' : (forall Γ Δ A, Γ ++ ϴ' ++ Δ ⊢ A [P] -> Γ ++ ϴ ++ Δ ⊢ A [P]) ->
+    forall Γ Δ A, Γ ++ (sg ϴ') :: Δ ⊧ □A -> Γ ++ sg ϴ :: Δ ⊧ □A.
+  Proof. intros H Γ Δ A; apply list_compose_monot_sg_mnd, logic_to_cl_ctx; assumption. Qed.
+
+  Lemma plogic_to_logic ϴ ϴ' : (forall Γ Δ A, Γ ++ (sg ϴ') :: Δ ⊧ □A -> Γ ++ sg ϴ :: Δ ⊧ □A) ->
+    forall Γ Δ A, Γ ++ ϴ' ++ Δ ⊢ A [P] -> Γ ++ ϴ ++ Δ ⊢ A [P].
+  Proof.
+  intros H Γ Δ A.
+  apply cl_ctx_to_logic.
+  apply (@list_compose_cons_sg_to_sem _ PMPS) in H; assumption.
+  Qed.
+
 
   Section Okada_Lemma.
 
     Notation ILLcl_closed := (@cl_closed _ _ _ CL_ctx).
     Notation ILLcl_increase := (@cl_increase _ _ CL_ctx).
+    Notation ILLcl_monotone := (@cl_monotone _ _ CL_ctx).
+    Notation ILLcl_le := (@cl_le _ _ _ CL_ctx).
+
+    Hint Resolve glb_in glb_out_l glb_out_r.
 
     Lemma Okada_var_1 X : sg (ivar X :: nil) ⊆ ⟦ivar X⟧.
     Proof. intros x Hx; subst; left; reflexivity. Qed.
@@ -243,7 +282,7 @@ Section SyntacticModel.
       apply gax_ir.
     Qed.
 
-    Lemma Okada_formula A : ((sg (A :: nil) ⊆ cl(⟦A⟧)) * (⟦A⟧ ⊆ ↓A))%type.
+    Lemma Okada_formula A : ((sg (A :: nil) ⊆ □(⟦A⟧)) * (⟦A⟧ ⊆ ↓A))%type.
     Proof.
     induction A; simpl;
       try (destruct IHA as [IHA01 IHA02]);
@@ -254,139 +293,101 @@ Section SyntacticModel.
            intros x Hx; inversion Hx; subst; constructor; auto; fail)]).
     - etransitivity; [ apply Okada_var_1 | apply ILLcl_increase ].
     - apply Okada_var_2.
-    - unfold ldual, rdual, ctx_orth.
-      intros x Hx [[de1 de2] A] Hy; subst; simpl.
-      constructor.
-      specialize Hy with nil; apply Hy; auto.
-    - transitivity (cl (cl (⟦ A1 ⟧) ∘ cl(⟦ A2 ⟧))).
-      + transitivity (cl_ctx (sg (A1 :: nil) ∘ sg (A2 :: nil))).
-        * unfold cl_ctx; simpl; unfold rdual, ctx_orth.
-          intros x Hx [[de1 de2] A] Hy; subst.
-          constructor.
-          specialize Hy with ((A1 :: nil) ++ A2 :: nil); apply Hy; auto.
-          split; auto.
-        * apply cl_monotone.
-          apply composes_monotone; assumption.
-      + apply (@cl_le _ _ _ CL_ctx).
-        apply cl_stable; auto.
-    - unfold magicwand_r.
-      etransitivity; [ | apply ILLcl_increase ].
-      intros x Hx y Hy [[G D] B] Hz; inversion Hy; subst; simpl.
-      apply lpam_ilr; auto.
-      assert (rdual ctx_orth (cl_ctx (⟦ A2 ⟧)) (G, D, B)) as Hz2
-        by (apply (fst (rtridual_eq ctx_orth _)); apply Hz).
-      change (A2 :: D) with ((A2 :: nil) ++ D); apply Hz2; auto.
+    - apply sg_subset, logic_to_cl_ctx, one_ilr.
+    - transitivity (cl (sg ((A1 :: nil) ++ A2 :: nil))).
+      + apply sg_subset, logic_to_cl_ctx, tens_ilr.
+      + apply ILLcl_le.
+        etransitivity; [ | apply cl_stable ]; auto.
+        simpl; change (A1 :: A2 :: nil) with ((A1 :: nil) ++ A2 :: nil).
+        apply sg_subset in IHA11; apply sg_subset in IHA21.
+        apply sg_subset; constructor; try assumption.
+    - transitivity (cl(sg(A2::nil)) ⟜ ↓A1).
+      + apply sg_subset.
+        intros x Hx; inversion Hx; subst.
+        apply logic_to_cl_ctx; intros; apply lpam_ilr; assumption.
+      + etransitivity; [ | apply ILLcl_increase ].
+        assert (Hmon := (@magicwand_r_monotone _ _ _ _ (@composes_monotone _ PScompose))); apply Hmon; auto.
+        apply ILLcl_le; assumption.
     - etransitivity; [ eapply (@cl_magicwand_r_3 _ _ _ CL_ctx) | ]; eauto.
-      intros x Hx; constructor.
-      apply ILLcl_closed in IHA22; auto.
-      apply IHA22, Hx; constructor; auto.
-    - unfold magicwand_r.
-      etransitivity; [ | apply ILLcl_increase ].
-      intros x Hx y Hy [[G D] B] Hz; inversion Hy; subst; simpl.
-      apply gen_pam_rule; auto.
-      change (N :: D) with ((N :: nil) ++ D); apply Hz.
-      apply (@Okada_var_1 atN); auto.
+      transitivity (↓A2 ⟜ sg(A1::nil)).
+      + assert (Hmon := (@magicwand_r_monotone _ _ _ _ (@composes_monotone _ PScompose))); apply Hmon; auto.
+        apply ILLcl_closed; auto.
+      + intros G HG; apply lpam_irr, HG; constructor; reflexivity.
+    - transitivity (cl(sg(N::nil)) ⟜ ↓A).
+      + apply sg_subset.
+        intros x Hx; inversion Hx; subst.
+        apply logic_to_cl_ctx; intros; apply gen_pam_rule; assumption.
+      + etransitivity; [ | apply ILLcl_increase ].
+        assert (Hmon := (@magicwand_r_monotone _ _ _ _ (@composes_monotone _ PScompose))); apply Hmon; auto.
+        apply ILLcl_monotone, Okada_var_1.
     - etransitivity; [ eapply (@cl_magicwand_r_3 _ _ _ CL_ctx) | ]; eauto.
-      intros x Hx; constructor.
-      assert (IHN := @Okada_var_2 atN).
-      apply ILLcl_closed in IHN; auto.
-      apply IHN, Hx; constructor; auto.
-    - unfold magicwand_l.
-      etransitivity; [ | apply ILLcl_increase ].
-      intros x Hx y Hy [[G D] B] Hz; inversion Hy; subst; simpl.
-      rewrite <- ? app_assoc; apply lmap_ilr; auto.
-      assert (rdual ctx_orth (cl_ctx (⟦ A2 ⟧)) (G, D, B)) as Hz2
-        by (apply (fst (rtridual_eq ctx_orth _)); apply Hz).
-      change (A2 :: D) with ((A2 :: nil) ++ D); apply Hz2; auto.
+      transitivity (↓N ⟜ sg(A::nil)).
+      + assert (Hmon := (@magicwand_r_monotone _ _ _ _ (@composes_monotone _ PScompose))); apply Hmon; auto.
+        apply ILLcl_closed, Okada_var_2; auto.
+      + intros G HG; apply gen_irr, HG; constructor; reflexivity.
+    - transitivity (↓A1 ⊸ cl(sg(A2::nil))).
+      + apply sg_subset.
+        intros x Hx; inversion Hx; subst.
+        apply logic_to_cl_ctx; intros; list_simpl; apply lmap_ilr; assumption.
+      + etransitivity; [ | apply ILLcl_increase ].
+        assert (Hmon := (@magicwand_l_monotone _ _ _ _ (@composes_monotone _ PScompose))); apply Hmon; auto.
+        apply ILLcl_le; assumption.
     - etransitivity; [ eapply (@cl_magicwand_l_3 _ _ _ CL_ctx) | ]; eauto.
-      intros x Hx; constructor.
-      apply ILLcl_closed in IHA22; auto.
-      apply IHA22, Hx.
-      change (A1 :: x) with ((A1 :: nil) ++ x); constructor; auto.
-    - unfold magicwand_l.
-      etransitivity; [ | apply ILLcl_increase ].
-      intros x Hx y Hy [[G D] B] Hz; inversion Hy; subst; simpl.
-      rewrite <- ? app_assoc; apply neg_map_rule; auto.
-      change (N :: D) with ((N :: nil) ++ D); apply Hz.
-      apply (@Okada_var_1 atN); auto.
+      transitivity (sg(A1::nil) ⊸ ↓A2).
+      + assert (Hmon := (@magicwand_l_monotone _ _ _ _ (@composes_monotone _ PScompose))); apply Hmon; auto.
+        apply ILLcl_closed; auto.
+      + intros G HG; apply lmap_irr, HG.
+        change (A1 :: G) with ((A1::nil) ++ G) ; constructor; reflexivity.
+    - transitivity (↓A ⊸ cl(sg(N::nil))).
+      + apply sg_subset.
+        intros x Hx; inversion Hx; subst.
+        apply logic_to_cl_ctx; intros; list_simpl; apply neg_map_rule; assumption.
+      + etransitivity; [ | apply ILLcl_increase ].
+        assert (Hmon := (@magicwand_l_monotone _ _ _ _ (@composes_monotone _ PScompose))); apply Hmon; auto.
+        apply ILLcl_monotone, Okada_var_1.
     - etransitivity; [ eapply (@cl_magicwand_l_3 _ _ _ CL_ctx) | ]; eauto.
-      intros x Hx; constructor.
-      assert (IHN := @Okada_var_2 atN).
-      apply ILLcl_closed in IHN; auto.
-      apply IHN, Hx.
-      change (A :: x) with ((A :: nil) ++ x); constructor; auto.
+      transitivity (sg(A::nil) ⊸ ↓N).
+      + assert (Hmon := (@magicwand_l_monotone _ _ _ _ (@composes_monotone _ PScompose))); apply Hmon; auto.
+        apply ILLcl_closed, Okada_var_2; auto.
+      + intros G HG; apply neg_irr, HG.
+        change (A :: G) with ((A::nil) ++ G) ; constructor; reflexivity.
     - etransitivity; [ | apply ILLcl_increase ].
       apply top_greatest.
-    - etransitivity; [ | apply ILLcl_increase ].
-      apply glb_in.
-      + apply cl_le in IHA11; auto.
-        etransitivity; [ | apply IHA11 ].
-        intros x Hx; subst.
-        unfold cl; simpl; unfold ldual, rdual, ctx_orth.
-        intros [[si1 si2] C] H; simpl.
-        apply with_ilr1.
-        specialize H with (A1 :: nil); apply H; auto.
-      + apply cl_le in IHA21; auto.
-        etransitivity; [ | apply IHA21 ].
-        intros x Hx; subst.
-        unfold cl; simpl; unfold ldual, rdual, ctx_orth.
-        intros [[si1 si2] C] H; simpl.
-        apply with_ilr2.
-        specialize H with (A2 :: nil); apply H; auto.
-    - unfold ldual, rdual, ctx_orth.
-      intros x Hx; inversion Hx; subst; constructor; auto.
-      + specialize X with (nil,nil,A1); list_simpl in X; apply X.
-        intros y Hy; list_simpl.
-        apply IHA12; auto.
-      + specialize X0 with (nil,nil,A2); list_simpl in X0; apply X0.
-        intros y Hy; list_simpl.
-        apply IHA22; auto.
+    - transitivity (cl (sg(A1 :: nil)) ∩ cl(sg(A2 :: nil))).
+      + apply glb_in; apply sg_subset, logic_to_cl_ctx; [ apply with_ilr1 | apply with_ilr2 ].
+      + etransitivity; [ | apply ILLcl_increase ].
+        apply (@mglb_monotone _ _ subset_preorder glb); auto; apply ILLcl_le; assumption.
+    - transitivity (cl(↓A1) ∩ cl(↓A2)).
+      + apply (@mglb_monotone _ _ subset_preorder glb);auto; apply ILLcl_monotone; assumption.
+      + etransitivity; [ apply (@mglb_monotone _ _ subset_preorder glb), dc_closed | ]; auto.
+        intros G [pi1 pi2]; apply with_irr; [ apply pi1 | apply pi2 ].
     - unfold ldual, rdual, ctx_orth.
       intros x Hx [[de1 de2] A] Hy; subst; simpl.
-      constructor.
-    - transitivity (lub (cl (⟦ A1 ⟧)) (cl(⟦ A2 ⟧))).
+      apply zero_ilr.
+    - transitivity (lub (sg (A1::nil)) (sg(A2::nil))).
       + intros x Hx [[de1 de2] A] Hy; subst; simpl.
         unfold rdual, ctx_orth, lub in Hy.
-        constructor.
-        * specialize Hy with (A1 :: nil); apply Hy; auto.
-        * specialize Hy with (A2 :: nil); apply Hy; auto.
-      + apply lub_out; auto.
-        * apply (@cl_idempotent _ _ CL_ctx).
-        * apply (@cl_monotone _ _ CL_ctx).
-          intros x; auto.
-        * apply (@cl_monotone _ _ CL_ctx).
-          intros x; auto.
-    - etransitivity; [ | apply ILLcl_increase ].
-      unfold ldual, rdual, ctx_orth.
-      apply glb_in; intros x Hx; subst.
-      + exists (A :: nil); reflexivity.
-      + enough (sg (!A :: nil) ⊆ cl(⟦A⟧)) as Hoc by (apply Hoc; reflexivity).
-        apply cl_le in IHA01; auto.
-        etransitivity; [ | apply IHA01 ].
-        intros x Hx; subst.
-        unfold cl; simpl; unfold ldual, rdual, ctx_orth.
-        intros [[si1 si2] C] H; simpl.
-        apply de_ilr.
-        specialize H with (A :: nil); apply H; auto.
-    - intros x Hx; inversion Hx; subst.
-      inversion H; subst.
-      constructor; auto.
-      unfold ldual, rdual, ctx_orth in X.
-      specialize X with (nil,nil,A); list_simpl in X; apply X.
-      intros y Hy; list_simpl.
-      apply IHA02; auto.
+        apply plus_ilr; cons2app; apply Hy; auto.
+      + apply lub_out; auto; [ apply (@cl_idempotent _ _ CL_ctx) | | ];
+          (etransitivity; [ eassumption | ]); apply ILLcl_monotone; intros ?; auto.
+    - etransitivity; [ | apply ILLcl_increase ]; apply glb_in.
+      + apply sg_subset; exists (A::nil); reflexivity.
+      + transitivity (cl (sg (A :: nil))).
+        * apply sg_subset, logic_to_cl_ctx; apply de_ilr.
+        * apply ILLcl_le; assumption.
+    - etransitivity; [ apply pre_store_monotone, ILLcl_monotone, IHA02 | ]; auto.
+      etransitivity; [ apply pre_store_monotone, dc_closed | ]; auto.
+      intros G [Hoc pi]; inversion Hoc; subst; apply oc_irr, pi.
     Qed.
-
-    Notation "⟬߭ Γ ⟭" := (list_form_presem PS_ctx (ILLval P) Γ) (at level 49).
 
     (* We lift the result to contexts, ie list of formulas *)
 
-    Lemma Okada_ctx Γ: cl (⟬߭Γ⟭)  Γ.
+    Lemma Okada_ctx Γ: □⟬߭Γ⟭ Γ.
     Proof.
-    induction Γ as [ | A ga Hga ]; unfold list_form_presem; simpl.
+    induction Γ as [ | A Γ HG ]; unfold list_form_presem; simpl.
     - apply ILLcl_increase; reflexivity.
     - apply (@cl_stable _ _ _ CL_ctx); auto.
-      change (A :: ga) with ((A :: nil) ++ ga); constructor; auto.
+      change (A :: Γ) with ((A :: nil) ++ Γ); constructor; auto.
       apply Okada_formula; auto.
     Qed.
 
@@ -405,18 +406,18 @@ Section cut_admissibility.
 
   (* Coercion: the phase model relying on cut-free provability over P is a phase model for P *)
   Instance PMILL_cfat : MPhaseModel P := {
-    PMPS := PS_ctx (cutupd_ipfrag P false);
-    PMval := ILLval (cutupd_ipfrag P false);
-    PMgax := @ILLgax (cutupd_ipfrag P false) P_gax_at_l P_gax_at_r P_gax_cut }.
+    PMPS := PS_ctx (cutrm_ipfrag P);
+    PMval := ILLval (cutrm_ipfrag P);
+    PMgax := @ILLgax (cutrm_ipfrag P) P_gax_at_l P_gax_at_r P_gax_cut }.
 
-  Theorem ill_cut_elimination Γ A : ill P Γ A -> ill (cutupd_ipfrag P false) Γ A.
+  Theorem ill_cut_elimination Γ A : ill P Γ A -> ill (cutrm_ipfrag P) Γ A.
   Proof.
     intros pi.
     apply (ill_soundness PMILL_cfat) in pi; auto.
-    assert (gax_noN_l (cutupd_ipfrag P false)) as HgaxN_cf by assumption.
-    assert (gax_at_l (cutupd_ipfrag P false)) as Hgax_at_l_cf by assumption.
-    assert (gax_at_r (cutupd_ipfrag P false)) as Hgax_at_r_cf by assumption.
-    assert (gax_cut (cutupd_ipfrag P false)) as Hgax_cut_cf by assumption.
+    assert (gax_noN_l (cutrm_ipfrag P)) as HgaxN_cf by assumption.
+    assert (gax_at_l (cutrm_ipfrag P)) as Hgax_at_l_cf by assumption.
+    assert (gax_at_r (cutrm_ipfrag P)) as Hgax_at_r_cf by assumption.
+    assert (gax_cut (cutrm_ipfrag P)) as Hgax_cut_cf by assumption.
     assert (HO := snd (Okada_formula HgaxN_cf Hgax_at_l_cf Hgax_at_r_cf Hgax_cut_cf A)).
     apply (@cl_closed _ _ _ PSCL) in HO; [ | apply dc_closed ].
     apply cl_le in pi.
